FEC/Verif_matrix.v
@@ -6,38 +6,12 @@ Require Import CommonVST.
 Require Import VandermondeList.
 Require Import Specs.
 Require Import Poly.
+Require Import FECTactics.
 
 Set Bullet Behavior "Strict Subproofs".
 
-Ltac solve_qpoly_bounds :=
-  let pose_bounds p :=
-    pose proof (modulus_poly_bound (proj1_sig p) (@ssrfun.svalP _ (fun y => deg y < deg mod_poly) p));
-    pose proof fec_n_eq; rep_lia in
-  let pose_mod_bounds p :=
-    pose proof (modulus_poly_bound (p %~ mod_poly) (pmod_lt_deg mod_poly p));
-    pose proof fec_n_eq; rep_lia in
-  match goal with
-  | [H: _ |- poly_to_int (proj1_sig ?p) <= ?x] => pose_bounds p
-  | [H: _ |- 0 <= poly_to_int (proj1_sig ?p) <= ?x] => pose_bounds p
-  | [H: _ |- 0 <= poly_to_int (proj1_sig ?p) < ?x] => pose_bounds p
-  | [H: _ |- poly_to_int (?p %~ mod_poly) <= ?x] => pose_mod_bounds p
-  | [H: _ |- 0 <= poly_to_int (?p %~ mod_poly) <= ?x] => pose_mod_bounds p
-  | [H: _ |- 0 <= poly_to_int (?p %~ mod_poly) < ?x] => pose_mod_bounds p
-  end.
 
-Ltac solve_wf :=
-  repeat(match goal with
-  | [H: _ |- wf_matrix (F:=F) (scalar_mul_row_partial (F:=F) _ _ _ _) _ _] => apply scalar_mul_row_partial_wf
-  | [H: _ |- wf_matrix (F:=F) (scalar_mul_row (F:=F) _ _ _) _ _ ] => apply scalar_mul_row_partial_wf
-  | [H: _ |- wf_matrix (F:=F) (all_cols_one_partial (F:=F) _ _ _) _ _ ] => apply all_cols_one_partial_wf
-  | [H: _ |- wf_matrix (F:=F) (add_multiple_partial (F:=F) _ _ _ _ _) _ _] => apply add_multiple_partial_wf
-  | [H: _ |- wf_matrix (F:=F) (add_multiple (F:=F) _ _ _ _ ) _ _] => apply add_multiple_partial_wf
-  | [H: _ |- wf_matrix (F:=F) (sub_all_rows_partial (F:=F) _ _ _ ) _ _] => apply sub_all_rows_partial_wf
-  | [H: _ |- wf_matrix (F:=F) (gauss_all_steps_rows_partial (F:=F) _ _ _ ) _ _] => apply gauss_all_steps_rows_partial_wf
-  | [H: _ |- wf_matrix (F:=F) (all_lc_one_rows_partial (F:=F) _ _ ) _ _] => apply all_lc_one_rows_partial_wf
-  | [H: _ |- wf_matrix (F:=F) (all_lc_one_rows_partial (F:=F) _ _ ) _ _] => apply all_lc_one_rows_partial_wf
-  end; try lia); assumption.
-
+(*
 (*Remove (Int.repr (Int.unsigned _)) and (Int.zero_ext) from qpolys*)
 Ltac rewrite_repr x :=
     let N := fresh in
@@ -59,12 +33,11 @@ Ltac rewrite_zbits_mod x :=
     assert (N: Zbits.Zzero_ext 8 (poly_to_int (x %~ mod_poly)) = poly_to_int (x %~ mod_poly)) by (
       rewrite Zbits.Zzero_ext_mod; [|rep_lia]; replace (two_p 8) with (256) by reflexivity;
       rewrite Zmod_small; [reflexivity | solve_qpoly_bounds]); rewrite -> N; clear N.
-
-
-
+*)
 
 Hint Rewrite fec_n_eq : rep_lia.
 Hint Rewrite fec_max_h_eq : rep_lia.
+
 
 (** Verification [fec_generate_weights]*)
 (*TODO: move after gaussian when done*)
@@ -73,25 +46,19 @@ Proof.
   pose proof (mod_poly_PosPoly) as Hpospoly.
   pose proof (mod_poly_PrimPoly) as Hprimpoly.
   start_function. freeze Ftrace := (data_at _ _ _ (gv _trace)).
-  forward_loop (EX (i : Z) (l: list (list Z)),
+    forward_loop (EX (i : Z) (l: list (list Z)),
     PROP (0 <= i <= fec_max_h /\ Zlength l = fec_max_h /\ Forall (fun x => Zlength x = fec_n - 1) l /\
-      forall (x: Z), 0 <= x < i -> (forall (y: Z), 0 <= y < fec_n - 1 -> Znth y (Znth x l) = 
+        forall (x: Z), 0 <= x < i -> (forall (y: Z), 0 <= y < fec_n - 1 -> Znth y (Znth x l) = 
         poly_to_int ((monomial (Z.to_nat (x * y)) %~ mod_poly ))))
     LOCAL (gvars gv; temp _i (Vint (Int.repr i)))
-    SEP (FRZL Ftrace;
-      data_at Ews (tarray tuchar fec_n) (power_to_index_contents fec_n) (gv _fec_2_index);
-      data_at Ews (tarray tuchar fec_n) index_to_power_contents (gv _fec_2_power);
-      data_at Ews (tarray tuchar fec_n) (inverse_contents fec_n) (gv _fec_invefec);
-      data_at Ews (tarray (tarray tuchar (fec_n - 1)) fec_max_h) (map_int_val_2d l) (gv _fec_weights)))
-   break:
+    SEP (FRZL Ftrace; FIELD_TABLES gv;
+        data_at Ews (tarray (tarray tuchar (fec_n - 1)) fec_max_h) (map_int_val_2d l) (gv _fec_weights)))
+    break:
       (PROP ()
       LOCAL (gvars gv)
-      SEP (data_at Ews tint (Vint (Int.zero)) (gv _trace);
-          data_at Ews (tarray tuchar fec_n) (power_to_index_contents fec_n) (gv _fec_2_index);
-          data_at Ews (tarray tuchar fec_n) index_to_power_contents (gv _fec_2_power);
-          data_at Ews (tarray tuchar fec_n) (inverse_contents fec_n) (gv _fec_invefec);
+      SEP (data_at Ews tint (Vint (Int.zero)) (gv _trace); FIELD_TABLES gv;
           data_at Ews (tarray (tarray tuchar (fec_n - 1)) fec_max_h) 
-          (rev_mx_val (weight_mx_list fec_max_h (fec_n - 1)))  (gv _fec_weights))).
+          (rev_mx_val (weight_mx_list fec_max_h (fec_n - 1)))  (gv _fec_weights))). 
   - forward. Exists 0%Z. Exists (list_repeat (Z.to_nat fec_max_h) (list_repeat (Z.to_nat (fec_n - 1)) 0%Z)).
     entailer!. split. rewrite Zlength_list_repeat'. rep_lia. rewrite Forall_forall. intros x Hin.
     apply in_list_repeat in Hin. subst. rewrite Zlength_list_repeat'. rep_lia. unfold map_int_val_2d.
@@ -102,19 +69,15 @@ Proof.
       (forall (x y: Z), (0 <= x < i /\ 0 <= y < fec_n - 1) \/ (x = i /\ 0 <= y < j) -> Znth y (Znth x l) = 
         poly_to_int ((monomial (Z.to_nat (x * y)) %~ mod_poly ))))
       LOCAL (gvars gv; temp _i (Vint (Int.repr i)); temp _j (Vint (Int.repr j)))
-      SEP (FRZL Ftrace; data_at Ews (tarray tuchar fec_n) (power_to_index_contents fec_n) (gv _fec_2_index);
-        data_at Ews (tarray tuchar fec_n) index_to_power_contents (gv _fec_2_power);
-        data_at Ews (tarray tuchar fec_n) (inverse_contents fec_n) (gv _fec_invefec);
-        data_at Ews (tarray (tarray tuchar (fec_n - 1)) fec_max_h) (map_int_val_2d l) (gv _fec_weights)))
+      SEP (FRZL Ftrace; FIELD_TABLES gv;
+           data_at Ews (tarray (tarray tuchar (fec_n - 1)) fec_max_h) (map_int_val_2d l) (gv _fec_weights)))
       break: (EX (l: list (list Z)),
         (PROP (Zlength l = fec_max_h /\ Forall (fun x => Zlength x = fec_n - 1) l /\
-        forall (x: Z), 0 <= x <= i -> (forall (y: Z), 0 <= y < fec_n - 1 -> Znth y (Znth x l) = 
-        poly_to_int ((monomial (Z.to_nat (x * y)) %~ mod_poly ))))
-      LOCAL (gvars gv; temp _i (Vint (Int.repr i)))
-      SEP (FRZL Ftrace; data_at Ews (tarray tuchar fec_n) (power_to_index_contents fec_n) (gv _fec_2_index);
-        data_at Ews (tarray tuchar fec_n) index_to_power_contents (gv _fec_2_power);
-        data_at Ews (tarray tuchar fec_n) (inverse_contents fec_n) (gv _fec_invefec);
-        data_at Ews (tarray (tarray tuchar (fec_n - 1)) fec_max_h) (map_int_val_2d l) (gv _fec_weights)))).
+          forall (x: Z), 0 <= x <= i -> (forall (y: Z), 0 <= y < fec_n - 1 -> Znth y (Znth x l) = 
+          poly_to_int ((monomial (Z.to_nat (x * y)) %~ mod_poly ))))
+        LOCAL (gvars gv; temp _i (Vint (Int.repr i)))
+        SEP (FRZL Ftrace; FIELD_TABLES gv;
+             data_at Ews (tarray (tarray tuchar (fec_n - 1)) fec_max_h) (map_int_val_2d l) (gv _fec_weights)))).
       * forward. Exists 0%Z. Exists l. entailer!. intros x y [Hbefore | Hcont]. apply H2; lia. lia.
       * Intros j. Intros lj. forward_if.
         -- (*Want to simplify the index*)
@@ -123,11 +86,10 @@ Proof.
               unfold Int.mods. rewrite !Int.signed_repr; try rep_lia. rewrite Z.rem_mod_nonneg by rep_lia.
               rewrite unsigned_repr; rep_lia. split. rep_lia. assert (i * j <= fec_max_h * (fec_n - 1)).
               apply Z.mul_le_mono_nonneg; lia. assert (fec_max_h * (fec_n - 1) = 32640). rewrite fec_max_h_eq.
-              rewrite fec_n_eq. reflexivity. rep_lia. }
+              rewrite fec_n_eq. reflexivity. rep_lia. } unfold FIELD_TABLES. Intros.
             forward.
           ++ entailer!. simpl. rewrite Hidx. assumption. 
-          ++ entailer!. rewrite Hidx. rewrite power_to_index_contents_Znth. simpl. 
-             rewrite_repr_mod (monomial (Z.to_nat ((i * j) mod 255))). solve_qpoly_bounds. assumption.            
+          ++ entailer!. rewrite Hidx. rewrite power_to_index_contents_Znth. simpl. simpl_repr. solve_qpoly_bounds.  assumption.            
           ++ entailer!. (*Why do I get this goal?*)
              destruct H23. apply repr_inj_signed in H24;  rep_lia.
           ++ simpl. rewrite Hidx. rewrite power_to_index_contents_Znth; [| assumption]. 
@@ -138,8 +100,7 @@ Proof.
               { entailer!. simpl. rewrite field_compatible_field_address. simpl. f_equal. rep_lia.
                 unfold field_compatible; simpl. 
                 destruct H21 as [Hptr [ Hleg [Hszcomp [Hal Hnest]]]]. simpl in *. repeat(split; auto); try rep_lia. }
-             forward. unfold Int.zero_ext. rewrite_repr_mod (monomial (Z.to_nat ((i * j) mod 255))).
-             rewrite_zbits_mod ((monomial (Z.to_nat ((i * j) mod 255)))). forward.
+             forward. simpl_repr. forward.
              Exists (j+1). Exists (upd_Znth i lj  (upd_Znth j (Znth i lj)
               (poly_to_int (monomial (Z.to_nat ((i * j) mod 255)) %~ mod_poly)))). entailer!. (*inner loop re establish invariant*)
             ** repeat(split).
@@ -157,63 +118,37 @@ Proof.
                   rewrite H6. rep_lia. apply Znth_In; rep_lia. }
                   destruct Hycase as [Hbefore | Hcurr].
                   rewrite upd_Znth_diff by rep_lia. apply H7; lia. 
-                  subst. rewrite upd_Znth_same by rep_lia. 
-                  (*The (somewhat) interesting part of the proof: x ^ (n % 255) = x ^ n (mod mod_poly)*)
-                  f_equal. pose proof (modulus_poly_primitive) as Hprim. unfold primitive in Hprim.
-                  destruct Hprim as [Hpos [Hirred [Hdiv Hinbound]]].
-                  rewrite modulus_poly_deg in Hdiv. rewrite fec_n_pow_2_nat in Hdiv.
-                  replace (255) with (fec_n - 1) by rep_lia. 
-                  assert(Hrem: (i * j) mod (fec_n - 1) = (i * j) - (fec_n - 1) * ((i * j) / (fec_n - 1))).
-                  rewrite (Z.div_mod (i * j) (fec_n - 1)) at 2. lia. rep_lia. rewrite Hrem.
-                  (*In order to get rid of the subtraction, we need to multiply the LHS by 1 - ie,
-                    monomial (fec_n - 1_ * (i * j / fec_n - 1))*)
-                   assert (0 <= (i * j / (fec_n - 1))). apply Z.div_pos. lia. rep_lia.
-                  assert (Hone: monomial (Z.to_nat ((fec_n - 1) * (i * j / (fec_n - 1)))) %~ mod_poly = one). {
-                  replace (Z.to_nat ((fec_n - 1) * (i * j / (fec_n - 1)))) with
-                    ((Z.to_nat (fec_n - 1)) * Z.to_nat (i * j / (fec_n - 1)))%nat by rep_lia.
-                  (*TODO: this should really be a separate lemma*)
-                  remember (Z.to_nat (i * j / (fec_n - 1))) as pow. clear Heqpow. induction pow. 
-                  rewrite Nat.mul_0_r. rewrite monomial_0. pose proof modulus_poly_deg. 
-                  rewrite pmod_refl; try lia. reflexivity. auto. apply (@deg_gt_one _ _ Hprimpoly).
-                  replace (Z.to_nat (fec_n - 1) * S pow)%nat with (Z.to_nat (fec_n - 1) + (Z.to_nat (fec_n - 1) * pow))%nat by rep_lia.
-                  rewrite <- monomial_exp_law. rewrite pmod_mult_distr by auto. rewrite IHpow. rewrite poly_mult_1_r.
-                  rewrite divides_pmod_iff in Hdiv. unfold divides_pmod in Hdiv. unfold nth_minus_one in Hdiv.
-                  rewrite <- pmod_cancel in Hdiv by auto. rewrite pmod_twice by auto.
-                  replace (Z.to_nat (fec_n - 1)) with (Z.to_nat fec_n - 1)%nat by rep_lia. rewrite Hdiv.
-                  rewrite pmod_refl; try lia. reflexivity. auto.  apply (@deg_gt_one _ _ Hprimpoly). 
-                  left. apply f_nonzero. auto.  }
-                  rewrite <- (poly_mult_1_r (monomial (Z.to_nat (i * j - (fec_n - 1) * (i * j / (fec_n - 1)))))).
-                  rewrite <- Hone. rewrite pmod_mult_reduce by auto. rewrite monomial_exp_law.
-                  f_equal. f_equal. rewrite <- Z2Nat.inj_add; try rep_lia. rewrite <- Hrem.
-                  pose proof (Z.mod_pos_bound (i * j) (fec_n - 1)). lia.
-              --- unfold Int.zero_ext. rewrite unsigned_repr; try rep_lia.
-                  rewrite zbits_small; try rep_lia. reflexivity.
+                  subst. rewrite upd_Znth_same by rep_lia. f_equal. apply (@monomial_powers_eq_mod _ _ Hprimpoly).
+                  rewrite Zmod_mod by lia. assert (Hfsz: Z.to_nat 255 = field_size mod_poly). {
+                  apply Nat2Z.inj. rewrite field_size_fec_n. rep_lia. } rewrite Hfsz. apply Nat.mod_mod; lia.
+              --- solve_repr_int. reflexivity. 
             ** unfold map_int_val_2d. rewrite <- !upd_Znth_map. rewrite !Znth_map. entailer!.
                rep_lia.
         -- (*end of inner loop*) forward. Exists lj. entailer!. intros x Hx y Hy.
            apply H7. rep_lia.
       * Intros lj. forward. Exists (i+1)%Z. Exists lj. entailer!. split.
         -- intros x Hx y Hy. apply H6; lia.
-        -- unfold Int.zero_ext. rewrite unsigned_repr; try rep_lia.  rewrite zbits_small; try rep_lia. reflexivity.
+        -- solve_repr_int. reflexivity. 
     + (*end of outer loop*) forward. entailer!.
       assert (Hweight: (map_int_val_2d l) = (rev_mx_val (weight_mx_list fec_max_h (fec_n - 1)))). {
-      unfold rev_mx_val. unfold map_int_val_2d. unfold rev_mx.
+      unfold rev_mx_val. unfold map_int_val_2d. unfold rev_mx. rewrite !map_map.
       apply Znth_eq_ext.
         - rewrite !Zlength_map. unfold weight_mx_list. rewrite prop_list_length. lia. rep_lia.
         - intros i' Hi'. rewrite Zlength_map in Hi'. rewrite H0 in Hi'.
           assert (Hfn: 0 <= fec_n - 1) by rep_lia. assert (Hfh: 0 <= fec_max_h) by rep_lia. 
           pose proof (weight_matrix_wf Hfn Hfh) as Hwf.
           destruct Hwf as [Hlen [Hn Hinlen]]. 
-          rewrite !Znth_map; try list_solve. f_equal. f_equal.
+          rewrite !Znth_map;[ | | list_solve]. f_equal. f_equal.
           unfold weight_mx_list. rewrite prop_list_Znth by rep_lia.
           apply Znth_eq_ext.
           + rewrite Zlength_rev. rewrite Zlength_map. rewrite prop_list_length. rewrite Forall_forall in H1.
             rewrite H1. reflexivity. apply Znth_In; try rep_lia. list_solve. 
           + intros j' Hj'. rewrite Forall_forall in H1. rewrite H1 in Hj'.
             2: { apply Znth_In; rep_lia. } rewrite Znth_rev.
-            rewrite !Znth_map. rewrite Zlength_map. rewrite prop_list_length.
-            rewrite prop_list_Znth. rewrite H2. f_equal. simpl. f_equal. f_equal. lia. rep_lia.
-            assumption. rep_lia. rep_lia. rewrite Zlength_map. rewrite prop_list_length; try rep_lia.
+            rewrite !Znth_map. rewrite Zlength_map. rewrite prop_list_length by rep_lia.
+            rewrite prop_list_Znth by rep_lia. rewrite H2. 
+            f_equal. simpl. f_equal. f_equal. lia. rep_lia. rep_lia.
+            rewrite Zlength_map. rewrite prop_list_length; try rep_lia.
             rewrite Zlength_map. rewrite prop_list_length; rep_lia.
           + rewrite <- Hlen in Hi'. apply Hi'. (*why doesn't rewrite work directly?*) }
       rewrite Hweight. cancel. thaw Ftrace. cancel. 
@@ -223,9 +158,8 @@ Proof.
     destruct Hwf' as [Hlen [Hn Hinlen]]. rewrite <- Forall_forall in Hinlen. 
     forward_call(gv, fec_max_h, fec_n - 1,  (weight_mx_list fec_max_h (fec_n - 1)),
       (gv _fec_weights)).
-    + entailer!.   simpl. f_equal. unfold Int.zero_ext. rewrite !unsigned_repr by rep_lia.
-      rewrite !zbits_small by rep_lia. repeat(f_equal); rep_lia.
-    + (*need the result about 2d and 1d arrays*)
+    + entailer!. simpl. f_equal. solve_repr_int. repeat(f_equal); rep_lia. 
+    +  (*need the result about 2d and 1d arrays*) unfold FIELD_TABLES.
       rewrite data_at_2darray_concat. unfold rev_mx_val. unfold map_int_val_2d. rewrite <- map_map.
       rewrite <- !concat_map. rewrite rev_concat_flatten. cancel.
       unfold rev_mx_val. unfold map_int_val_2d. unfold rev_mx. rewrite !Zlength_map.
@@ -251,7 +185,7 @@ Proof.
         rewrite !map_map. rewrite in_map_iff. intros [x [Hx Hin]]. subst.
         rewrite !Zlength_map. rewrite Zlength_rev. rewrite Zlength_map. apply Hinlen'. assumption.
       * auto.
-Qed. 
+Qed.
       
 (** Verification of [fec_matrix_transform]*)
 
@@ -262,21 +196,15 @@ Proof.
     PROP (0 <= k <= m)
     LOCAL (temp _k (Vint (Int.repr (k))); temp _p s; temp _i_max (Vint (Int.repr m)); temp _j_max (Vint (Int.repr n));
       gvars gv)
-    SEP(data_at Ews (tarray tuchar fec_n) (power_to_index_contents fec_n) (gv _fec_2_index);
-   data_at Ews (tarray tuchar fec_n) index_to_power_contents (gv _fec_2_power);
-   data_at Ews (tarray tuchar fec_n) (inverse_contents fec_n) (gv _fec_invefec);
-   data_at Ews (tarray tuchar (m * n))
-     (map Vint (map Int.repr (flatten_mx 
-        (gauss_all_steps_rows_partial mx m k )))) s))
-    break: (PROP ()
-           LOCAL (temp _p s; temp _i_max (Vint (Int.repr m)); temp _j_max (Vint (Int.repr n));
-      gvars gv)
-            SEP(data_at Ews (tarray tuchar fec_n) (power_to_index_contents fec_n) (gv _fec_2_index);
-   data_at Ews (tarray tuchar fec_n) index_to_power_contents (gv _fec_2_power);
-   data_at Ews (tarray tuchar fec_n) (inverse_contents fec_n) (gv _fec_invefec);
-   data_at Ews (tarray tuchar (m * n))
-     (map Vint (map Int.repr (flatten_mx 
-        (gauss_all_steps_rows_partial mx m m )))) s)). 
+    SEP(FIELD_TABLES gv;
+        data_at Ews (tarray tuchar (m * n)) (map Vint (map Int.repr (flatten_mx 
+          (gauss_all_steps_rows_partial mx m k )))) s))
+    break: (
+      PROP ()
+      LOCAL (temp _p s; temp _i_max (Vint (Int.repr m)); temp _j_max (Vint (Int.repr n)); gvars gv)
+      SEP(FIELD_TABLES gv;
+          data_at Ews (tarray tuchar (m * n)) (map Vint (map Int.repr (flatten_mx   
+            (gauss_all_steps_rows_partial mx m m )))) s)). 
 { forward. Exists 0%Z. entailer!. }
 { Intros k. forward_if.
   { (*body of outer loop *) 
@@ -285,46 +213,23 @@ Proof.
     (EX (i : Z),
       PROP (0 <= i <= m)
       LOCAL (temp _i (Vint (Int.repr i)); temp _k (Vint (Int.repr k)); temp _p s; 
-      temp _i_max (Vint (Int.repr m)); temp _j_max (Vint (Int.repr n)); gvars gv)
-      SEP (data_at Ews (tarray tuchar fec_n) (power_to_index_contents fec_n) (gv _fec_2_index);
-        data_at Ews (tarray tuchar fec_n) index_to_power_contents (gv _fec_2_power);
-        data_at Ews (tarray tuchar fec_n) (inverse_contents fec_n) (gv _fec_invefec);
-        data_at Ews (tarray tuchar (m * n)) (map Vint (map Int.repr 
-          (flatten_mx (all_cols_one_partial 
+             temp _i_max (Vint (Int.repr m)); temp _j_max (Vint (Int.repr n)); gvars gv)
+      SEP (FIELD_TABLES gv;
+        data_at Ews (tarray tuchar (m * n)) (map Vint (map Int.repr (flatten_mx (all_cols_one_partial 
             (gauss_all_steps_rows_partial (F:=F) mx m k) k i )))) s))
-      break: (PROP ()
+      break: (
+        PROP ()
         LOCAL (temp _k (Vint (Int.repr k)); temp _p s; 
-      temp _i_max (Vint (Int.repr m)); temp _j_max (Vint (Int.repr n)); gvars gv)
-      SEP (data_at Ews (tarray tuchar fec_n) (power_to_index_contents fec_n) (gv _fec_2_index);
-        data_at Ews (tarray tuchar fec_n) index_to_power_contents (gv _fec_2_power);
-        data_at Ews (tarray tuchar fec_n) (inverse_contents fec_n) (gv _fec_invefec);
-        data_at Ews (tarray tuchar (m * n)) (map Vint (map Int.repr 
-          (flatten_mx (all_cols_one_partial 
-            (gauss_all_steps_rows_partial (F:=F) mx m k) k m )))) s)).
+               temp _i_max (Vint (Int.repr m)); temp _j_max (Vint (Int.repr n)); gvars gv)
+        SEP (FIELD_TABLES gv;
+             data_at Ews (tarray tuchar (m * n)) (map Vint (map Int.repr (flatten_mx (all_cols_one_partial 
+                (gauss_all_steps_rows_partial (F:=F) mx m k) k m )))) s)).
     { forward. Exists 0%Z. entailer!. }
     { Intros i. forward_if.
-      { forward. (*Want to simplify pointer in q*)
-        assert_PROP ((force_val (sem_binary_operation' Osub (tptr tuchar) tint
-          (eval_binop Oadd (tptr tuchar) tuchar (eval_binop Oadd (tptr tuchar) tint s
-           (eval_binop Omul tuchar tuchar (Vint (Int.repr i))
-           (Vint (Int.repr n)))) (Vint (Int.repr n))) (Vint (Int.repr 1)))) =
-           (offset_val (((i * n) + n) - 1) s)). { entailer!.
-        rewrite sem_sub_pi_offset; auto. rep_lia. }
-        rewrite H3. clear H3.
+      { forward. (*simplify q*) pointer_to_offset s. 
         forward.
         { entailer!. rewrite sem_sub_pi_offset; auto; try rep_lia. }
-        { (*Now, we will simplify pointer in m*)
-          assert_PROP ((force_val
-               (sem_binary_operation' Oadd (tptr tuchar) tint
-                  (eval_binop Osub (tptr tuchar) tuchar (offset_val (i * n + n - 1) s)
-                     (Vint (Int.repr n))) (Vint (Int.repr 1)))) =
-            offset_val (i * n) s). { entailer!.
-          rewrite sem_sub_pi_offset; auto; try rep_lia. f_equal. simpl. rewrite sem_add_pi_ptr_special; auto;
-          try rep_lia. simpl. rewrite offset_offset_val. f_equal. lia. }
-          rewrite H3; clear H3.
-          assert_PROP ((offset_val (i * n) s) = field_address (tarray tuchar (m * n)) 
-            (SUB ((i * n) + n - 1 - (n-1))) s). { entailer!. rewrite arr_field_address; auto.
-            simpl. f_equal. lia. apply (matrix_bounds_within); lia. } rewrite H3; rename H3 into Hm_offset. 
+        { pointer_to_offset_with s (i * n).  (*Now, we will simplify pointer in m*)
           forward.
           assert (Hwf' : wf_matrix (F:=F) (all_cols_one_partial (F:=F) 
             (gauss_all_steps_rows_partial (F:=F) mx m k) k i) m n) by solve_wf.
@@ -339,9 +244,7 @@ Proof.
            temp _i (Vint (Int.repr i)); temp _k (Vint (Int.repr k)); 
            temp _p s; temp _i_max (Vint (Int.repr m)); temp _j_max (Vint (Int.repr n)); 
            gvars gv)
-           SEP (data_at Ews (tarray tuchar fec_n) (power_to_index_contents fec_n) (gv _fec_2_index);
-           data_at Ews (tarray tuchar fec_n) index_to_power_contents (gv _fec_2_power);
-           data_at Ews (tarray tuchar fec_n) (inverse_contents fec_n) (gv _fec_invefec);
+           SEP (FIELD_TABLES gv;
            data_at Ews (tarray tuchar (m * n))
              (map Vint
                 (map Int.repr
@@ -349,36 +252,26 @@ Proof.
                       (all_cols_one_partial (F:=F) (gauss_all_steps_rows_partial (F:=F) mx m k)
                          k i)))) s))) as x.
          forward_loop x break: x; subst. (*so I don't have to write it twice*)
-        { entailer!. }
-        { assert_PROP (force_val (sem_sub_pi tuchar Signed 
-            (offset_val (i * n + n - 1) s) (Vint (Int.repr k))) =
-            offset_val (i * n + n - 1 - k) s). { entailer!.
-           rewrite sem_sub_pi_offset;auto. simpl. f_equal. lia. rep_lia. }
-           (*TODO: will need more general stuff probably*)
-           assert (0 <= i * n + n - 1 - k < m * n). {
-            apply matrix_bounds_within; lia. }
+        { entailer!. solve_offset. } 
+        {  assert (0 <= i * n + n - 1 - k < m * n). {
+            apply matrix_bounds_within; lia. } 
            assert_PROP (force_val (sem_sub_pi tuchar Signed 
             (offset_val (i * n + n - 1) s) (Vint (Int.repr k))) =
-            field_address (tarray tuchar (m * n)) (SUB  (i * n + n - 1 - k)) s). {
-            entailer!. rewrite H3. rewrite arr_field_address; auto. simpl. f_equal. lia. }
-            clear H3. 
+            field_address (tarray tuchar (m * n)) (SUB  (i * n + n - 1 - k)) s). { entailer!. solve_offset. }  
            assert_PROP ((0 <= i * n + n - 1 - k <
               Zlength (map Int.repr (flatten_mx
               (all_cols_one_partial (F:=F) (gauss_all_steps_rows_partial (F:=F) mx m k)
               k i))))). {
-           entailer!. list_solve. } simpl_reptype. rewrite Zlength_map in H3.
+           entailer!. list_solve. } simpl_reptype. rewrite Zlength_map in H5.
            forward.
-          { entailer!. rewrite (@flatten_mx_Znth m n); try lia. 
-            pose proof (qpoly_int_bound (get (F:=F) (all_cols_one_partial (F:=F) 
-                (gauss_all_steps_rows_partial (F:=F) mx m k) k i) 
-                i k)).  rewrite Int.unsigned_repr; rep_lia. assumption. }
-          { entailer!. rewrite sem_sub_pi_offset; auto. rep_lia. }
+          { entailer!. rewrite (@flatten_mx_Znth m n); try lia. simpl_repr. solve_qpoly_bounds. solve_wf. } 
+          { entailer!. solve_offset. }
           { forward_if.
             { (*contradiction due to [strong_inv]*)
               assert (Znth (i * n + n - 1 - k)
                 (flatten_mx (all_cols_one_partial (F:=F) (gauss_all_steps_rows_partial (F:=F) mx m k)
                 k i)) <> 0%Z). {
-              rewrite (@flatten_mx_Znth m n); try lia. 2: assumption. intro Hzero.
+              rewrite (@flatten_mx_Znth m n); [ |assumption | lia | lia]. intro Hzero.
               rewrite poly_to_int_zero_iff in Hzero. 
               assert (Hrm : 0 <= k < m) by lia.
               assert (Hcm : 0 <= i < m) by lia.
@@ -389,8 +282,7 @@ Proof.
               unfold q0. unfold r0. exist_eq.
               simpl in Hzero. assumption. } 
               apply mapsto_memory_block.repr_inj_unsigned in H6. contradiction. 2: rep_lia.
-              rewrite (@flatten_mx_Znth m n); try lia. eapply Z_expand_bounds.
-              3 : { apply qpoly_int_bound. } lia. rep_lia. assumption. }
+              rewrite (@flatten_mx_Znth m n); try lia. solve_qpoly_bounds. assumption.  }
             { forward. entailer!. }
           }
         }
@@ -398,85 +290,60 @@ Proof.
          assert_PROP (force_val (sem_sub_pi tuchar Signed 
             (offset_val (i * n + n - 1) s) (Vint (Int.repr k))) =
             field_address (tarray tuchar (m * n)) (SUB  (i * n + n - 1 - k)) s). {
-            entailer!. rewrite sem_sub_pi_offset;auto. simpl. rewrite arr_field_address; auto. simpl. f_equal. lia.
-            apply matrix_bounds_within; lia. rep_lia. } 
-         assert (0 <= i * n + n - 1 - k < m * n). {
-            apply matrix_bounds_within; lia. }
+            entailer!. solve_offset. }
+         assert (0 <= i * n + n - 1 - k < m * n) by nia. 
          assert_PROP ((0 <= i * n + n - 1 - k <
           Zlength (map Int.repr (flatten_mx
          (all_cols_one_partial (F:=F) (gauss_all_steps_rows_partial (F:=F) mx m k) k i))))). 
          entailer!. list_solve. rewrite Zlength_map in H5.
          (*Doing some stuff to simplify here so we don't need to repeat this in each branch*)
-         pose proof (Hpolybound:= (qpoly_int_bound (get (F:=F) (all_cols_one_partial (F:=F) 
-                (gauss_all_steps_rows_partial (F:=F) mx m k) k i) i k))).
-          forward; try rewrite (@flatten_mx_Znth m n); try lia; try assumption.
-        { entailer!. lia. }
-        { entailer!. rewrite sem_sub_pi_offset; auto. rep_lia. }
-        { forward.
-          { entailer!. }
-          { entailer!. rewrite inverse_contents_Znth. rewrite poly_of_int_inv.
-            simpl. unfold poly_inv. rewrite unsigned_repr. all: solve_qpoly_bounds. } 
+          forward; try (rewrite (@flatten_mx_Znth m n); try lia; try assumption).
+        { entailer!. simpl_repr. solve_qpoly_bounds. }
+        { entailer!. solve_offset.  }
+        { unfold FIELD_TABLES. Intros. (*need for "forward"*)
+          assert ((Int.min_signed <= poly_to_int (proj1_sig (get (F:=F) 
+            (all_cols_one_partial (F:=F) (gauss_all_steps_rows_partial (F:=F) mx m k) k i) i k)) <=
+            Int.max_signed)) by solve_qpoly_bounds. forward.
+          { entailer!. solve_qpoly_bounds. }
+          { entailer!. rewrite inverse_contents_Znth. rewrite poly_of_int_inv. simpl. 
+            unfold poly_inv. rewrite unsigned_repr. all: solve_qpoly_bounds. } 
           { forward. forward. (*simplify before for loop*)
-            rewrite inverse_contents_Znth. 2: solve_qpoly_bounds. rewrite poly_of_int_inv. simpl.
+            rewrite inverse_contents_Znth by solve_qpoly_bounds. rewrite poly_of_int_inv. simpl. 
             remember (get (F:=F) (all_cols_one_partial (F:=F)
                       (gauss_all_steps_rows_partial (F:=F) mx m k) k i) i k) as qij eqn : Hqij. 
-            (*remember (proj1_sig qij) as pij eqn : Hpij.*)
             remember (find_inv mod_poly qij) as qij_inv eqn : Hqinv.
             replace (poly_inv mod_poly (proj1_sig qij)) with (proj1_sig qij_inv). 2 : {
-            unfold poly_inv. rewrite poly_to_qpoly_unfold. rewrite Hqinv. reflexivity. }
-            unfold Int.zero_ext.
-            rewrite_repr qij_inv. rewrite_zbits qij_inv.
-            rewrite unsigned_repr; [| rep_lia]. rewrite zbits_small; [| rep_lia].
-            assert_PROP ((force_val
-               (sem_add_ptr_int tuchar Signed (offset_val (i * n + n - 1) s)
-                  (Vint (Int.repr 1)))) = offset_val (i * n + n) s). { entailer!.
-            f_equal. lia. } rewrite H6; clear H6.
-            assert (Hmn_leq: 0 <= i * n + n <= m * n). { split; try lia. 
-              replace n with (1 * n) at 2 by lia. rewrite <- Z.mul_add_distr_r.
-              apply Z.mul_le_mono_nonneg_r; lia. } 
+            unfold poly_inv. rewrite poly_to_qpoly_unfold. rewrite Hqinv. reflexivity. } simpl_repr.
+            solve_repr_int. pointer_to_offset_with s (i * n + n). (*simplify pointer in n*)
+            assert (Hmn_leq: 0 <= i * n + n <= m * n) by nia. 
             (*Scalar multiplication loop*)
-            (*Unfortunately, lots of duplication here: can we save locals in a variable?*)
-            forward_loop (EX (j : Z),
-            PROP (0 <= j <= n)
-            LOCAL (temp _inv (Vint (Int.repr (poly_to_int (proj1_sig qij_inv))));
+            (*Lots of duplication here, so we save the locals in a variable*)
+            remember [temp _inv (Vint (Int.repr (poly_to_int (proj1_sig qij_inv))));
               temp _t'11 (Vint (Int.repr (poly_to_int (proj1_sig qij_inv))));
               temp _t'10 (Vint (Int.repr (poly_to_int (proj1_sig qij))));
               temp _w (Vint (Int.repr i));
               temp _m (field_address (tarray tuchar (m * n)) [ArraySubsc (i * n + n - 1 - (n - 1))] s);
-              (*temp _q (field_address (tarray tuchar (m * n)) [ArraySubsc (cols_one_row * n + n - 1)] s);*)
-              temp _q (offset_val (i * n + n - 1) s);
               temp _i (Vint (Int.repr i)); temp _k (Vint (Int.repr k)); 
               temp _p s; temp _i_max (Vint (Int.repr m)); temp _j_max (Vint (Int.repr n)); 
-              gvars gv;
-              temp _n (field_address0 (tarray tuchar (m * n)) (SUB (i * n + n - j)) s))
-              (*temp _n (offset_val (cols_one_row * n + n - 1 - j) s))*)
-            SEP (data_at Ews (tarray tuchar fec_n) (power_to_index_contents fec_n) (gv _fec_2_index);
-                 data_at Ews (tarray tuchar fec_n) index_to_power_contents (gv _fec_2_power);
-                 data_at Ews (tarray tuchar fec_n) (inverse_contents fec_n) (gv _fec_invefec);
+              gvars gv ] as LOCALS.
+            forward_loop (EX (j : Z),
+            PROP (0 <= j <= n)
+            (LOCALx (
+              temp _n (field_address0 (tarray tuchar (m * n)) (SUB (i * n + n - j)) s) ::
+              temp _q (offset_val (i * n + n - 1) s) :: LOCALS)
+            (SEP (FIELD_TABLES gv;
                  data_at Ews (tarray tuchar (m * n)) (map Vint (map Int.repr
-                  (flatten_mx (scalar_mul_row_partial (all_cols_one_partial (F:=F) 
-                    (gauss_all_steps_rows_partial (F:=F) mx m k) k i) 
-                    i qij_inv j)))) s))
+                    (flatten_mx (scalar_mul_row_partial (all_cols_one_partial (F:=F) 
+                    (gauss_all_steps_rows_partial (F:=F) mx m k) k i)  i qij_inv j)))) s))%assert5))
             break: (PROP ()
-              LOCAL (temp _inv (Vint (Int.repr (poly_to_int (proj1_sig qij_inv))));
-              temp _t'11 (Vint (Int.repr (poly_to_int (proj1_sig qij_inv))));
-              temp _t'10 (Vint (Int.repr (poly_to_int (proj1_sig qij))));
-              temp _w (Vint (Int.repr i));
-              temp _m (field_address (tarray tuchar (m * n)) [ArraySubsc (i * n + n - 1 - (n - 1))] s); 
-              temp _q (field_address (tarray tuchar (m * n)) [ArraySubsc (i * n + n - 1)] s);
-              temp _i (Vint (Int.repr i)); temp _k (Vint (Int.repr k)); 
-              temp _p s; temp _i_max (Vint (Int.repr m)); temp _j_max (Vint (Int.repr n)); 
-              gvars gv)
-              SEP (data_at Ews (tarray tuchar fec_n) (power_to_index_contents fec_n) (gv _fec_2_index);
-                 data_at Ews (tarray tuchar fec_n) index_to_power_contents (gv _fec_2_power);
-                 data_at Ews (tarray tuchar fec_n) (inverse_contents fec_n) (gv _fec_invefec);
-                 data_at Ews (tarray tuchar (m * n)) (map Vint (map Int.repr
-                  (flatten_mx (scalar_mul_row (all_cols_one_partial (F:=F) 
-                    (gauss_all_steps_rows_partial (F:=F) mx m k) k i) 
-                    i qij_inv)))) s)).
-            { Exists 0%Z. entailer!. rewrite arr_field_address0; auto. simpl. f_equal; lia.
-              rewrite scalar_mul_row_partial_0. cancel. }
-            { Intros j. assert (Hcn : 0 <= i * n). { apply Z.mul_nonneg_nonneg; lia. } 
+              (LOCALx (temp _q (field_address (tarray tuchar (m * n)) [ArraySubsc (i * n + n - 1)] s) :: LOCALS)
+              (SEP (FIELD_TABLES gv;
+                    data_at Ews (tarray tuchar (m * n)) (map Vint (map Int.repr
+                    (flatten_mx (scalar_mul_row (all_cols_one_partial (F:=F) 
+                    (gauss_all_steps_rows_partial (F:=F) mx m k) k i) i qij_inv)))) s)))%assert5).
+            { Exists 0%Z. rewrite HeqLOCALS. entailer!. solve_offset. 
+              rewrite scalar_mul_row_partial_0. unfold FIELD_TABLES. cancel.  }
+            { Intros j. assert (Hcn : 0 <= i * n). { apply Z.mul_nonneg_nonneg; lia. } rewrite HeqLOCALS.
               forward_if.
               { rewrite !arr_field_address0; auto. rewrite arr_field_address; auto.
                 rewrite isptr_denote_tc_test_order; auto. unfold test_order_ptrs.
@@ -492,46 +359,43 @@ Proof.
                   entailer!.
                 - apply matrix_bounds_within; lia.
                 - lia. }
-              { forward. entailer!. apply field_address0_isptr. apply arr_field_compatible0; auto; try lia.
+              { forward. entailer!. solve_offset.
                 assert_PROP ((field_address (tarray tuchar (m * n)) 
                     [ArraySubsc (i * n + n - 1 - (n - 1))] s) =
                     (field_address0 (tarray tuchar (m * n)) [ArraySubsc (i * n + n - 1 - (n - 1))] s)). {
-                entailer!. rewrite <- Hm_offset. rewrite arr_field_address0; auto. f_equal; simpl; lia. lia. }
-                rewrite H8 in H7; clear H8.
-                assert_PROP (j < n). { entailer!. apply ptr_comparison_gt_iff in H7; auto. all: simpl; lia. }
-                clear H7.
+                entailer!. solve_offset. } 
+                rewrite H9 in H8; clear H9.
+                assert_PROP (j < n). { entailer!. apply ptr_comparison_gt_iff in H8; auto. all: simpl; lia. }
+                clear H8.
                 assert_PROP ((force_val
                 (sem_binary_operation' Osub (tptr tuchar) tint
                   (field_address0 (tarray tuchar (m * n)) [ArraySubsc (i * n + n - j)] s)
                   (Vint (Int.repr 1)))) = 
                 (field_address (tarray tuchar (m * n)) [ArraySubsc (i * n + n - 1 - j)] s)). {
                 entailer!. rewrite !arr_field_address0; auto; try lia.
-                rewrite !arr_field_address; auto; try lia. rewrite sem_sub_pi_offset; auto; try rep_lia.
-                f_equal; simpl; lia. } rewrite H7; clear H7. 
+                rewrite !arr_field_address; auto; try lia. solve_offset. } rewrite H8; clear H8. 
                 (*Need length bound also*)
                 assert_PROP (0 <= i * n + n - 1 - j < Zlength (map Int.repr
                 (flatten_mx (scalar_mul_row_partial (F:=F)
                 (all_cols_one_partial (F:=F) (gauss_all_steps_rows_partial (F:=F) mx m k) k i) i qij_inv j)))).
                  { entailer!. list_solve. }
-                rewrite Zlength_map in H7.
+                rewrite Zlength_map in H8.
                 assert (Hwf'' : wf_matrix (F:=F) (scalar_mul_row_partial (F:=F)
                   (all_cols_one_partial (F:=F) (gauss_all_steps_rows_partial (F:=F) mx m k) k i) i qij_inv j) m n)
                 by solve_wf.
                 forward.
-                - entailer!. rewrite (@flatten_mx_Znth m n); try lia.
-                  rewrite unsigned_repr; solve_qpoly_bounds. auto. 
+                - entailer!. rewrite (@flatten_mx_Znth m n); try lia. simpl_repr. solve_qpoly_bounds. auto.
                 - rewrite (@flatten_mx_Znth m n); try lia; auto.
                   remember ((get (F:=F)
                            (scalar_mul_row_partial (F:=F)
                               (all_cols_one_partial (F:=F) (gauss_all_steps_rows_partial (F:=F) mx m k)
                                  k i) i qij_inv j) i j)) as aij.
                   forward_call.
-                  + rewrite_repr aij. rewrite_repr qij_inv. rewrite_zbits aij. rewrite_zbits qij_inv. split; solve_qpoly_bounds.
-                  + (*simplify result of function call*)
-                    rewrite_repr aij. rewrite_repr qij_inv. rewrite_zbits aij. rewrite_zbits qij_inv.
-                    rewrite !poly_of_int_inv. forward. Exists (j+1). entailer!.
-                    rewrite arr_field_address; auto; try lia.
-                    rewrite arr_field_address0; auto; try lia. f_equal; lia.
+                  + unfold FIELD_TABLES. entailer!.
+                  + simpl_repr. split; solve_qpoly_bounds. 
+                  + (*simplify result of function call*) simpl_repr.
+                    rewrite !poly_of_int_inv. forward. Exists (j+1). rewrite HeqLOCALS. entailer!. solve_offset.
+                    unfold FIELD_TABLES. cancel. 
                     rewrite !upd_Znth_map. (*need to simplify the scalar_mult*)
                     rewrite (@scalar_mul_row_plus_1 F _ m n). simpl_reptype.
                     remember ((scalar_mul_row_partial (F:=F) (all_cols_one_partial (F:=F)
@@ -548,98 +412,70 @@ Proof.
                      rewrite Heqmx'. rewrite (@scalar_mul_row_outside _ m n); try lia. reflexivity.
                      auto. } rewrite Hget. clear Hget. rewrite poly_mult_comm.
                       rewrite <- (@flatten_mx_set m n). simpl. cancel. all: try lia; auto. } 
-              { (*scalar mul loop return*) forward. entailer!.
-                - rewrite arr_field_address; auto; try lia. f_equal; simpl; lia. 
+              { (*scalar mul loop return*) forward. rewrite HeqLOCALS; entailer!.
+                - solve_offset.
                 - assert_PROP ((field_address (tarray tuchar (m * n)) 
                     [ArraySubsc (i * n + n - 1 - (n - 1))] s) =
                     (field_address0 (tarray tuchar (m * n)) [ArraySubsc (i * n + n - 1 - (n - 1))] s)). {
-                  entailer!. rewrite <- Hm_offset. rewrite arr_field_address0; auto. f_equal; simpl; lia. lia. }
-                  rewrite H29 in H7; clear H29.
+                  entailer!. solve_offset. }
+                  rewrite H21 in H8; clear H21.
                   (*need to know that j = n at end of loop*)
-                  assert (Hjn: j >= n). { 
-                    assert (Hft: forall a b, typed_false a b -> ~(typed_true a b)). { intros a b F T.
-                    unfold typed_true in T; unfold typed_false in F; rewrite T in F; inversion F. }
-                    apply Hft in H7; clear Hft. rewrite (not_iff_compat) in H7. 2: {
-                    rewrite ptr_comparison_gt_iff. reflexivity. all: auto. all: simpl; lia. }
-                    lia. } 
-                  assert (j = n) by lia. subst; clear Hjn H7. unfold scalar_mul_row. 
+                  assert (Hjn: j >= n). { apply typed_false_not_true in H8. rewrite (not_iff_compat) in H8.
+                  2: { rewrite ptr_comparison_gt_iff. reflexivity. all: auto. all: simpl; lia. }
+                  lia. } 
+                  assert (j = n) by lia. subst; clear Hjn H8. unfold scalar_mul_row. 
                   assert (Hlenn: (Zlength (Znth i (all_cols_one_partial (F:=F)
                           (gauss_all_steps_rows_partial (F:=F) mx m k) k i))) = n).
                   { destruct Hwf' as [Hlen [Hn' Hin]]. apply Hin.
                     apply Znth_In; lia. } rewrite Hlenn; cancel. } }
             (*no idea what level I'm on - coqide has stopped highlighting brackets, but at end of col loop*)
-            forward. Exists (i + 1). entailer!.
-            { f_equal. unfold Int.zero_ext. f_equal. rewrite unsigned_repr; 
-             [ rewrite zbits_small; [reflexivity | rep_lia] | rep_lia]. }
-            { rewrite all_cols_one_plus_1; try lia. 
+            rewrite HeqLOCALS; forward. Exists (i + 1). entailer!.
+            { solve_repr_int. reflexivity.  }
+            { rewrite all_cols_one_plus_1 by lia. 
               replace (ssralg.GRing.inv (R:=ssralg.GRing.Field.unitRingType F)) with (find_inv mod_poly) by reflexivity.
               rewrite (@all_cols_one_outside F m n); try lia. cancel. solve_wf. } } } } } }
       (*now we are completely finishing the col loop*)
     { forward. entailer!. replace (i) with m by lia. cancel. } }
   { (*start of second part: add kth row to all other rows*)
-    forward. (*simplify r*)
-    assert_PROP ((force_val (sem_binary_operation' Osub (tptr tuchar) tint
-                  (eval_binop Oadd (tptr tuchar) tuchar (eval_binop Oadd (tptr tuchar) tint s
-                  (eval_binop Omul tuchar tuchar (Vint (Int.repr k))
-                  (Vint (Int.repr n)))) (Vint (Int.repr n))) (Vint (Int.repr 1)))) = 
-                 offset_val (k * n + n - 1) s). { entailer!.
-    rewrite sem_sub_pi_offset; auto. rep_lia. } rewrite H1; clear H1.
+    forward. (*simplify r*) pointer_to_offset s.
     (*can't use [forward_for_simple_bound] because it cases i to a tuchar*)
-    (*TODO: again, lots of duplication*)
+    remember [temp _r (offset_val (k * n + n - 1) s); temp _k (Vint (Int.repr k)); 
+              temp _p s; temp _i_max (Vint (Int.repr m)); temp _j_max (Vint (Int.repr n)); 
+              gvars gv] as LOCALS.
     forward_loop (EX (i : Z),
       PROP (0 <= i <= m)
-      LOCAL  (temp _r (offset_val (k * n + n - 1) s); temp _k (Vint (Int.repr k));
-              temp _p s; temp _i_max (Vint (Int.repr m)); temp _j_max (Vint (Int.repr n)); temp _i (Vint (Int.repr i));
-              gvars gv)
-      SEP (data_at Ews (tarray tuchar fec_n) (power_to_index_contents fec_n) (gv _fec_2_index);
-            data_at Ews (tarray tuchar fec_n) index_to_power_contents (gv _fec_2_power);
-            data_at Ews (tarray tuchar fec_n) (inverse_contents fec_n) (gv _fec_invefec);
-            data_at Ews (tarray tuchar (m * n)) (map Vint (map Int.repr (flatten_mx
-          (sub_all_rows_partial (all_cols_one_partial (F:=F) (gauss_all_steps_rows_partial (F:=F) mx m k) k m) k i)))) s))
+      (LOCALx  (temp _i (Vint (Int.repr i)) :: LOCALS)
+      (SEP (FIELD_TABLES gv;
+            data_at Ews (tarray tuchar (m * n)) (map Vint (map Int.repr (flatten_mx (sub_all_rows_partial 
+           (all_cols_one_partial (F:=F) (gauss_all_steps_rows_partial (F:=F) mx m k) k m) k i)))) s))%assert5))
       break: 
       (PROP ()
-      LOCAL  (temp _r (offset_val (k * n + n - 1) s); temp _k (Vint (Int.repr k));
-              temp _p s; temp _i_max (Vint (Int.repr m)); temp _j_max (Vint (Int.repr n));
-              gvars gv)
-      SEP (data_at Ews (tarray tuchar fec_n) (power_to_index_contents fec_n) (gv _fec_2_index);
-            data_at Ews (tarray tuchar fec_n) index_to_power_contents (gv _fec_2_power);
-            data_at Ews (tarray tuchar fec_n) (inverse_contents fec_n) (gv _fec_invefec);
-            data_at Ews (tarray tuchar (m * n)) (map Vint (map Int.repr (flatten_mx
-          (sub_all_rows_partial (all_cols_one_partial (F:=F) (gauss_all_steps_rows_partial (F:=F) mx m k) k m) k m)))) s)).
+      (LOCALx  (LOCALS)
+      (SEP (FIELD_TABLES gv;
+            data_at Ews (tarray tuchar (m * n)) (map Vint (map Int.repr (flatten_mx (sub_all_rows_partial 
+            (all_cols_one_partial (F:=F) (gauss_all_steps_rows_partial (F:=F) mx m k) k m) k m)))) s))%assert5)).
     { (*initialization of subtract all rows loop*) 
-      forward. Exists 0%Z. entailer!. }
+      rewrite HeqLOCALS; forward. Exists 0%Z. rewrite HeqLOCALS; entailer!. }
     { (*Body of subtract all rows loop *) 
-      Intros i. forward_if.
+      Intros i. rewrite HeqLOCALS; forward_if.
       { (*i < m (loop body)*) 
         forward_if (PROP ()
-            LOCAL ( temp _r (offset_val (k * n + n - 1) s);
-              temp _k (Vint (Int.repr k)); temp _p s; temp _i_max (Vint (Int.repr m));
-              temp _j_max (Vint (Int.repr n)); temp _i (Vint (Int.repr i)); gvars gv)
-            SEP (data_at Ews (tarray tuchar fec_n) (power_to_index_contents fec_n) (gv _fec_2_index);
-             data_at Ews (tarray tuchar fec_n) index_to_power_contents (gv _fec_2_power);
-             data_at Ews (tarray tuchar fec_n) (inverse_contents fec_n) (gv _fec_invefec);
+            (LOCALx (temp _i (Vint (Int.repr i)) :: LOCALS)
+            (SEP (FIELD_TABLES gv;
              data_at Ews (tarray tuchar (m * n))
                (map Vint (map Int.repr (flatten_mx (if Z.eq_dec i k then
                 (sub_all_rows_partial (F:=F)(all_cols_one_partial (F:=F) 
                   (gauss_all_steps_rows_partial (F:=F) mx m k) k m) k i) else
                (add_multiple_partial (sub_all_rows_partial (F:=F)(all_cols_one_partial (F:=F) 
                   (gauss_all_steps_rows_partial (F:=F) mx m k) k m) k i) k i (q1 (f:=mod_poly)) n)
-                )))) s)). 
+                )))) s))%assert5)). 
         { (*when i != k*)
-          forward. (*simplify q*)
-          assert_PROP ((force_val (sem_binary_operation' Osub (tptr tuchar) tint
-            (eval_binop Oadd (tptr tuchar) tuchar (eval_binop Oadd (tptr tuchar) tint s
-            (eval_binop Omul tuchar tuchar (Vint (Int.repr i)) (Vint (Int.repr n))))
-            (Vint (Int.repr n))) (Vint (Int.repr 1)))) =
-            offset_val (i * n + n - 1) s). { entailer!. rewrite sem_sub_pi_offset; auto. rep_lia. }
-          rewrite H4; clear H4.
+          forward. (*simplify q*) pointer_to_offset s.
           forward_for (fun (j : Z) => PROP (0 <= j <= n)
             LOCAL (temp _q (offset_val (i * n + n - 1) s); temp _r (offset_val (k * n + n - 1) s);
               temp _k (Vint (Int.repr k)); temp _p s; temp _i_max (Vint (Int.repr m));
               temp _j_max (Vint (Int.repr n)); temp _i (Vint (Int.repr i)); temp _j (Vint (Int.repr j)); gvars gv)
-            SEP (data_at Ews (tarray tuchar fec_n) (power_to_index_contents fec_n) (gv _fec_2_index);
-             data_at Ews (tarray tuchar fec_n) index_to_power_contents (gv _fec_2_power);
-             data_at Ews (tarray tuchar fec_n) (inverse_contents fec_n) (gv _fec_invefec);
+            SEP (FIELD_TABLES gv;
              data_at Ews (tarray tuchar (m * n))
                (map Vint (map Int.repr (flatten_mx
                (add_multiple_partial (sub_all_rows_partial (F:=F)(all_cols_one_partial (F:=F) 
@@ -649,43 +485,37 @@ Proof.
            { entailer!. }
            { rename x into j. (*simplify *(q-j)*)
              assert_PROP (force_val (sem_sub_pi tuchar Signed (offset_val (i * n + n - 1) s) (Vint (Int.repr j))) =
-                offset_val (i * n + n - 1 - j) s). { entailer!.  rewrite sem_sub_pi_offset; auto. simpl.
-                f_equal; rep_lia. rep_lia. }
+                offset_val (i * n + n - 1 - j) s). { entailer!. solve_offset.  }
              assert_PROP (offset_val (i * n + n - 1 - j) s = 
-              field_address (tarray tuchar (m * n)) (SUB (i * n + n - 1 - j)) s). { entailer!.
-                rewrite arr_field_address; auto; try lia. simpl. f_equal; lia. apply matrix_bounds_within; lia. }
-             rewrite H6 in H5. (*TODO: can we automate this? *)
+              field_address (tarray tuchar (m * n)) (SUB (i * n + n - 1 - j)) s). { entailer!. solve_offset. }
+             rewrite H6 in H5.
              assert (Hij: 0 <= i * n + n - 1 - j < m * n) by (apply matrix_bounds_within; lia).
              assert_PROP ((0 <= i * n + n - 1 - j < Zlength (map Int.repr (flatten_mx (add_multiple_partial (F:=F)
               (sub_all_rows_partial (F:=F) (all_cols_one_partial (F:=F) 
               (gauss_all_steps_rows_partial (F:=F) mx m k) k m) k i) k i
               (q1 (f:=mod_poly)) j))))). { entailer!. list_solve. }
             rewrite Zlength_map in H7. forward.
-            { entailer!. rewrite (@flatten_mx_Znth m n); try lia. rewrite unsigned_repr; solve_qpoly_bounds.
-              solve_wf. }
-            { entailer!. rewrite H5. rewrite <- H6. auto. }
+            { entailer!. rewrite (@flatten_mx_Znth m n); try lia. simpl_repr. solve_qpoly_bounds. solve_wf. }
+            { entailer!. solve_offset. }
             { (*Simplify *(r-j) *)
-              rewrite (@flatten_mx_Znth m n); try lia. 2: solve_wf.
+              rewrite (@flatten_mx_Znth m n); [ | solve_wf | lia | lia].
               assert_PROP (force_val (sem_sub_pi tuchar Signed (offset_val (k * n + n - 1) s) (Vint (Int.repr j))) =
-                 offset_val (k * n + n - 1 - j) s). { entailer!. rewrite sem_sub_pi_offset; auto. simpl.
-               f_equal; rep_lia. rep_lia. }
+                 offset_val (k * n + n - 1 - j) s). { entailer!. solve_offset. }
               assert_PROP (offset_val (k * n + n - 1 - j) s = field_address (tarray tuchar (m * n))
-                (SUB (k * n + n - 1 - j)) s). { entailer!. rewrite arr_field_address; auto; try lia.
-              simpl; f_equal; lia. apply matrix_bounds_within; lia. } rewrite H9 in H8. 
+                (SUB (k * n + n - 1 - j)) s). { entailer!. solve_offset. }  rewrite H9 in H8. 
               assert (Hkj : 0 <= k * n + n - 1 - j < m * n) by (apply matrix_bounds_within; lia).
               assert_PROP ((0 <= k * n + n - 1 - j < Zlength (map Int.repr (flatten_mx
               (add_multiple_partial (F:=F)  (sub_all_rows_partial (F:=F)(all_cols_one_partial (F:=F) 
               (gauss_all_steps_rows_partial (F:=F) mx m k) k m) k i) k i 
               (q1 (f:=mod_poly)) j))))). { entailer!. list_solve. } rewrite Zlength_map in H10.
               forward.
-              { entailer!. rewrite (@flatten_mx_Znth m n); try lia. rewrite unsigned_repr; solve_qpoly_bounds.
-              solve_wf. }
-              { entailer!. rewrite H8. rewrite <- H9. auto. }
+              { entailer!. rewrite (@flatten_mx_Znth m n); try lia. simpl_repr. solve_qpoly_bounds. solve_wf.  }
+              { entailer!. solve_offset. }
               { (*actual subtraction*) 
-                rewrite (@flatten_mx_Znth m n); try lia. 2: solve_wf. forward.
-                { entailer!. rewrite H5; rewrite <- H6; auto. }
+                rewrite (@flatten_mx_Znth m n); [ | solve_wf | lia | lia]. forward.
+                { entailer!. solve_offset. }
                 { (*need lots of simplification*)
-                  unfold Int.xor. rewrite !unsigned_repr; try solve_qpoly_bounds.
+                  unfold Int.xor. simpl_repr. (*rewrite !unsigned_repr; try solve_qpoly_bounds.*)
                   rewrite xor_poly_to_int.
                   remember (add_multiple_partial (F:=F) (sub_all_rows_partial (F:=F)
                            (all_cols_one_partial (F:=F) (gauss_all_steps_rows_partial (F:=F) mx m k) k m) k i) k i
@@ -693,16 +523,14 @@ Proof.
                   forward. 
                   (*end of subtraction loop*)
                   Exists (j+1). entailer!.
-                  { f_equal. unfold Int.zero_ext. f_equal. 
-                    rewrite unsigned_repr; [ rewrite zbits_small; rep_lia | rep_lia]. } 
-                  { rewrite (@add_multiple_partial_plus_1 _ m n); try lia. 2: solve_wf.
-                    rewrite <- (@flatten_mx_set m n); try lia. 2: solve_wf.
+                  { solve_repr_int. reflexivity. } 
+                  { rewrite (@add_multiple_partial_plus_1 _ m n); try lia; [| solve_wf]. 
+                    rewrite <- (@flatten_mx_set m n); [| solve_wf | lia | lia].
                     rewrite ssralg.GRing.mul1r. 
                     replace (ssralg.GRing.add (V:=ssralg.GRing.Field.zmodType F)) with (qadd (f:=mod_poly)) by reflexivity.
-                    unfold qadd. unfold r_add. simpl. unfold poly_add_mod. simpl_reptype.
-                    (*TODO: fix spelling*)
-                    rewrite (@add_multiple_partial_outside _ m n); try lia. 2: solve_wf.
-                    rewrite (@add_multiple_partial_other_row _ m n); try lia. 2: solve_wf.
+                    unfold qadd. unfold r_add. unfold poly_add_mod. simpl_reptype.
+                    rewrite (@add_multiple_partial_outside _ m n); try lia; [| solve_wf].
+                    rewrite (@add_multiple_partial_other_row _ m n); try lia; [ | solve_wf].
                     (*We can get rid of the other [add_multiple_add_partial] since i <> k*)
                     remember ((proj1_sig  (get (F:=F)
                       (sub_all_rows_partial (F:=F) 
@@ -712,28 +540,24 @@ Proof.
                     as sum. 
                     (*now we just need to show the two pieces are equal*)
                      rewrite <- !upd_Znth_map. 
-                    assert (Hsum: Int.zero_ext 8 (Int.repr (poly_to_int sum)) = 
-                        (Int.repr (poly_to_int (sum %~ mod_poly)))). {
-                     unfold Int.zero_ext. f_equal.
-                     assert (Hdeg: deg sum < deg mod_poly). { rewrite Heqsum.
-                     eapply Z.le_lt_trans. apply poly_add_deg_max. apply Z.max_lub_lt;
+                    assert (Hdeg: deg sum < deg mod_poly). { rewrite Heqsum.
+                    eapply Z.le_lt_trans. apply poly_add_deg_max. apply Z.max_lub_lt;
                      apply (@ssrfun.svalP _ (fun y => deg y < deg mod_poly)). }
-                     rewrite pmod_refl; auto.
-                     apply modulus_poly_bound in Hdeg. 
-                     rewrite Zbits.Zzero_ext_mod; [|lia]. replace (two_p 8) with (256) by reflexivity.
-                     pose proof fec_n_bound; rewrite Zmod_small; rewrite unsigned_repr; rep_lia. 
-                     apply mod_poly_PosPoly. } rewrite Hsum. cancel. }
+                    assert (Hsum_bound: 0 <= (poly_to_int sum) < fec_n). {
+                     apply modulus_poly_bound in Hdeg. assumption. } solve_repr_int. simpl.
+                     rewrite (pmod_refl mod_poly sum); auto. cancel. }
                 }
               }
             }
           }
-          { (*end of subtraction loop*) entailer!. destruct (Z.eq_dec i k); try lia. rename x into j. replace j with n by lia. cancel. }
+          { (*end of subtraction loop*) rewrite HeqLOCALS; entailer!. destruct (Z.eq_dec i k); try lia.
+            rename x into j. replace j with n by lia. cancel. }
         }
         { (*i = k case (easier)*)
-           forward. entailer!. destruct (Z.eq_dec k k); try lia. cancel. }
-        { (*postcondition of sub_all_rows loop*) forward. Exists (i+1). entailer!.
-          { f_equal. unfold Int.zero_ext. f_equal. rewrite unsigned_repr; [rewrite zbits_small ; rep_lia | rep_lia]. } 
-          { rewrite sub_all_rows_plus_1; try lia. 
+           forward. rewrite HeqLOCALS; entailer!. destruct (Z.eq_dec k k); try lia. cancel. }
+        { (*postcondition of sub_all_rows loop*) rewrite HeqLOCALS; forward. Exists (i+1). rewrite HeqLOCALS; entailer!.
+          { solve_repr_int. reflexivity. }
+          { rewrite sub_all_rows_plus_1 by lia.
             replace (ssralg.GRing.opp (V:=ssralg.GRing.Ring.zmodType (ssralg.GRing.Field.ringType F))
                       (ssralg.GRing.one (ssralg.GRing.Field.ringType F))) with
               (q1 (f:=mod_poly)) by reflexivity. 
@@ -744,12 +568,11 @@ Proof.
             destruct Hwf' as [Hlen [Hn Hin]]. rewrite Hin. cancel. apply Znth_In. lia. }
             }
           }
-          { (*end of sub all rows loop*) forward. entailer!. replace i with m by lia. cancel. }
+          { (*end of sub all rows loop*) forward. rewrite HeqLOCALS; entailer!. replace i with m by lia. cancel. }
         }
         { (*postcondition of gauss_one_step loop*)
-          forward. Exists (k+1). entailer!.
-          { f_equal. unfold Int.zero_ext. f_equal.
-            rewrite unsigned_repr; [rewrite zbits_small ; rep_lia | rep_lia]. }
+          rewrite HeqLOCALS; forward. Exists (k+1). entailer!.
+          { solve_repr_int. reflexivity.  }
           { rewrite gauss_all_steps_rows_partial_plus_1. cancel. lia. }
         }
       }
@@ -764,64 +587,44 @@ Proof.
       PROP (0 <= i <= m - 1)
       LOCAL (temp _p s; temp _i_max (Vint (Int.repr m)); temp _j_max (Vint (Int.repr n)); temp _i (Vint (Int.repr i));
             gvars gv)
-      SEP (data_at Ews (tarray tuchar fec_n) (power_to_index_contents fec_n) (gv _fec_2_index);
-           data_at Ews (tarray tuchar fec_n) index_to_power_contents (gv _fec_2_power);
-           data_at Ews (tarray tuchar fec_n) (inverse_contents fec_n) (gv _fec_invefec);
-           data_at Ews (tarray tuchar (m * n))
-            (map Vint (map Int.repr (flatten_mx (all_lc_one_rows_partial 
-              (gauss_all_steps_rows_partial (F:=F) mx m m) i)))) s))
+      SEP (FIELD_TABLES gv;
+           data_at Ews (tarray tuchar (m * n)) (map Vint (map Int.repr (flatten_mx (all_lc_one_rows_partial 
+            (gauss_all_steps_rows_partial (F:=F) mx m m) i)))) s))
       break:
        (PROP ()
         LOCAL (temp _p s; temp _i_max (Vint (Int.repr m)); temp _j_max (Vint (Int.repr n)); gvars gv) 
-        SEP (data_at Ews (tarray tuchar fec_n) (power_to_index_contents fec_n) (gv _fec_2_index);
-           data_at Ews (tarray tuchar fec_n) index_to_power_contents (gv _fec_2_power);
-           data_at Ews (tarray tuchar fec_n) (inverse_contents fec_n) (gv _fec_invefec);
-           data_at Ews (tarray tuchar (m * n))
-            (map Vint (map Int.repr (flatten_mx (all_lc_one_rows_partial 
-              (gauss_all_steps_rows_partial (F:=F) mx m m) (m-1))))) s)).
+        SEP (FIELD_TABLES gv;
+           data_at Ews (tarray tuchar (m * n)) (map Vint (map Int.repr (flatten_mx (all_lc_one_rows_partial 
+            (gauss_all_steps_rows_partial (F:=F) mx m m) (m-1))))) s)).
     { (*initialization*) forward. Exists 0%Z. entailer!. }
     { (*outer loop for lc's 1*) Intros i. forward_if.
       { (*loop body*) forward.
-        (*simplify q*) assert_PROP ((force_val (sem_binary_operation' Osub (tptr tuchar) tint
-        (eval_binop Oadd (tptr tuchar) tuchar (eval_binop Oadd (tptr tuchar) tint s
-        (eval_binop Omul tuchar tuchar (Vint (Int.repr i)) (Vint (Int.repr n))))
-        (Vint (Int.repr n))) (Vint (Int.repr 1)))) = offset_val (i * n + n - 1) s). {
-        entailer!. rewrite sem_sub_pi_offset; auto. rep_lia. } rewrite H1; clear H1.
+        (*simplify q*) pointer_to_offset s. 
         assert_PROP (offset_val (i * n + n - 1) s = field_address (tarray tuchar (m * n)) (SUB (i * n + n - 1)) s). {
-        entailer!. rewrite arr_field_address; auto. simpl. f_equal; lia.
-        replace (i * n + n - 1) with (i * n + n - 1 - 0) by lia. apply matrix_bounds_within; lia. }
+        entailer!. solve_offset. }
         forward.
-        { entailer!. rewrite sem_sub_pi_offset; auto. rep_lia. }
-        { (*simplify m*) assert_PROP (force_val
-               (sem_binary_operation' Oadd (tptr tuchar) tint
-                  (eval_binop Osub (tptr tuchar) tuchar (offset_val (i * n + n - 1) s)
-                     (Vint (Int.repr n))) (Vint (Int.repr 1))) = offset_val (i * n + n - 1 - (n - 1)) s). {
-          entailer!. rewrite sem_sub_pi_offset; auto. simpl. rewrite sem_add_pi'; auto.
-          rewrite offset_offset_val. simpl; f_equal; lia. rep_lia. rep_lia. } rewrite H2; clear H2. 
+        { entailer!. solve_offset.  }
+        { (*simplify m*) pointer_to_offset_with s (i * n + n - 1 - (n - 1)).  
           assert_PROP (offset_val (i * n + n - 1 - (n - 1)) s = field_address (tarray tuchar (m * n))
-            (SUB ( i * n + n - 1 - ( n - 1))) s). { entailer!. rewrite arr_field_address; auto.
-          f_equal. simpl. lia. apply matrix_bounds_within; lia. } rewrite H2. 
+            (SUB ( i * n + n - 1 - ( n - 1))) s). { entailer!. solve_offset. } rewrite H2. 
           (*simplify (q-i)*) 
           assert_PROP (force_val (sem_sub_pi tuchar Signed (offset_val (i * n + n - 1) s) (Vint (Int.repr i))) =
-            field_address (tarray tuchar (m * n)) (SUB (i * n + n - 1 - i)) s). { entailer!.
-          rewrite sem_sub_pi_offset; auto. rewrite arr_field_address; auto. simpl. f_equal; lia.
-          apply matrix_bounds_within; lia. rep_lia. }
+            field_address (tarray tuchar (m * n)) (SUB (i * n + n - 1 - i)) s). { entailer!. solve_offset. }
           (*Also need length info in context*)
           assert_PROP ((0 <= i * n + n - 1 - i < Zlength (map Int.repr
             (flatten_mx (all_lc_one_rows_partial (F:=F) (gauss_all_steps_rows_partial (F:=F) mx m m) i))))). {
           entailer!. assert (0 <= i * n + n - 1 - i < m * n). apply matrix_bounds_within; lia. list_solve. }
           rewrite Zlength_map in H4. forward.
-          { (*pointer access is valid*) entailer!. rewrite (@flatten_mx_Znth m n); try lia. 2: solve_wf.
-            rewrite unsigned_repr; solve_qpoly_bounds. }
-          { entailer!. rewrite sem_sub_pi_offset; auto. rep_lia. }
+          { (*pointer access is valid*) entailer!. rewrite (@flatten_mx_Znth m n); [ | solve_wf | lia | lia].
+            simpl_repr. solve_qpoly_bounds. }
+          { entailer!. solve_offset. }
           { rewrite (@flatten_mx_Znth m n); [| solve_wf | lia |lia ].
             pose proof (Hpolybound:= (qpoly_int_bound (get (F:=F) (all_lc_one_rows_partial (F:=F) 
-                  (gauss_all_steps_rows_partial (F:=F) mx m m) i) i i))).
+                  (gauss_all_steps_rows_partial (F:=F) mx m m) i) i i))). unfold FIELD_TABLES. Intros.
             forward.
             { entailer!. }
-            { entailer!. rewrite inverse_contents_Znth; [| solve_qpoly_bounds]. simpl.
-              rewrite poly_of_int_inv. unfold poly_inv.
-              rewrite unsigned_repr; solve_qpoly_bounds. }
+            { entailer!. rewrite inverse_contents_Znth; [| solve_qpoly_bounds]. simpl. 
+              rewrite poly_of_int_inv. unfold poly_inv. simpl_repr. solve_qpoly_bounds. }
             { rewrite inverse_contents_Znth; [| solve_qpoly_bounds]. rewrite poly_of_int_inv.
               remember ((get (F:=F)(all_lc_one_rows_partial (F:=F) 
                 (gauss_all_steps_rows_partial (F:=F) mx m m) i) i i)) as aii.
@@ -829,15 +632,9 @@ Proof.
               remember (find_inv mod_poly aii) as aii_inv eqn : Haiiinv.
               replace (poly_inv mod_poly (proj1_sig aii)) with (proj1_sig aii_inv). 2 : {
               unfold poly_inv. rewrite poly_to_qpoly_unfold. rewrite Haiiinv. reflexivity. }
-              unfold Int.zero_ext. rewrite_repr aii_inv. rewrite_zbits aii_inv.
-              forward.
-              (*simplify n*)
-              assert_PROP (force_val (sem_binary_operation' Oadd (tptr tuchar) tint (offset_val (i * n + n - 1) s)
-                  (Vint (Int.repr 1))) = offset_val (i * n + n) s). { entailer!. f_equal; lia. }
-              rewrite H5; clear H5.
-              assert (Himn: 0 <= i * n + n <= m * n). { split; try lia. replace (i * n + n) with ((i+1) * n) by lia.
-              apply Z.mul_le_mono_nonneg_r; lia. }
-              assert (Hin0: 0 <= i * n). { apply Z.mul_nonneg_nonneg; lia. }
+              simpl_repr. forward. pointer_to_offset_with s (i * n + n).
+              assert (Himn: 0 <= i * n + n <= m * n) by nia. 
+              assert (Hin0: 0 <= i * n) by nia.
               (*inner loop (scalar multiply)*)
               forward_loop (EX (j: Z),
                 PROP (0 <= j <= n)
@@ -848,13 +645,11 @@ Proof.
                   temp _m (field_address (tarray tuchar (m * n)) [ArraySubsc (i * n + n - 1 - (n - 1))] s);
                   temp _q (offset_val (i * n + n - 1) s); temp _p s; temp _i_max (Vint (Int.repr m));
                   temp _j_max (Vint (Int.repr n)); temp _i (Vint (Int.repr i)); gvars gv)
-                SEP (data_at Ews (tarray tuchar fec_n) (power_to_index_contents fec_n) (gv _fec_2_index);
-                  data_at Ews (tarray tuchar fec_n) index_to_power_contents (gv _fec_2_power);
-                  data_at Ews (tarray tuchar fec_n) (inverse_contents fec_n) (gv _fec_invefec);
+                SEP (FIELD_TABLES gv;
                   data_at Ews (tarray tuchar (m * n))(map Vint (map Int.repr
                     (flatten_mx (scalar_mul_row_partial 
                       (all_lc_one_rows_partial (F:=F) (gauss_all_steps_rows_partial (F:=F) mx m m) i) i aii_inv j)))) s)).
-              { Exists 0%Z. entailer!. rewrite arr_field_address0; auto. simpl. f_equal; lia.
+              { Exists 0%Z. entailer!. solve_offset. unfold FIELD_TABLES. 
                 rewrite scalar_mul_row_partial_0. cancel.  }
               { entailer!. assert (Hbound: 0 <= (i * n + n - j) <= m * n) by lia. 
                 rewrite !arr_field_address0; auto. rewrite arr_field_address; auto.
@@ -870,20 +665,18 @@ Proof.
                   instantiate (1 := sizeof tuchar * (i * n + n - 1 - (n - 1))). simpl. lia. entailer!.
                 - apply matrix_bounds_within; lia. } 
               { forward.
-                { entailer!. rewrite arr_field_address0; auto. lia. }
+                { entailer!. solve_offset. }
                 { (*simplify if condition*)
                   assert_PROP (field_address (tarray tuchar (m * n)) [ArraySubsc (i * n + n - 1 - (n - 1))] s = 
                     (field_address0 (tarray tuchar (m * n)) [ArraySubsc (i * n + n - 1 - (n - 1))] s)). { entailer!.
-                  rewrite arr_field_address; auto; try lia. rewrite arr_field_address0; auto; try lia. }
-                  rewrite H6 in HRE; clear H6.
+                  solve_offset. } rewrite H6 in HRE; clear H6.
                   assert_PROP (j < n). { entailer!. 
                    rewrite ptr_comparison_gt_iff in HRE; auto; simpl; lia. } rename H6 into Hjn; clear HRE.
                   (*simplify n so we can dereference*)
                    assert_PROP ((force_val (sem_binary_operation' Osub (tptr tuchar) tint
                   (field_address0 (tarray tuchar (m * n)) [ArraySubsc (i * n + n - j)] s)
                   (Vint (Int.repr 1)))) = field_address (tarray tuchar (m * n)) (SUB (i * n + n - 1 - j)) s). {
-                  entailer!. rewrite arr_field_address0; auto; try lia. rewrite sem_sub_pi_offset; auto; try rep_lia.
-                  rewrite arr_field_address; auto; try lia. f_equal; simpl; lia. } rewrite H6; clear H6.
+                  entailer!. rewrite arr_field_address0; auto; try lia. solve_offset. }  rewrite H6; clear H6.
                   (*length goal*)
                   assert_PROP (0 <= i * n + n - 1 - j < Zlength (map Int.repr
                     (flatten_mx (scalar_mul_row_partial (F:=F)  (all_lc_one_rows_partial (F:=F) 
@@ -892,18 +685,18 @@ Proof.
                    list_solve. }
                   rewrite Zlength_map in H6. 
                   forward.
-                  { entailer!. rewrite (@flatten_mx_Znth m n); try lia. 2: solve_wf.
-                    rewrite unsigned_repr; solve_qpoly_bounds. }
+                  { entailer!. rewrite (@flatten_mx_Znth m n); [| solve_wf | lia | lia]. simpl_repr. 
+                    solve_qpoly_bounds. }
                   { rewrite (@flatten_mx_Znth m n); [ | solve_wf | lia | lia].
                     remember ((get (F:=F)(scalar_mul_row_partial (F:=F)  (all_lc_one_rows_partial (F:=F)
                               (gauss_all_steps_rows_partial (F:=F) mx m m) i) i aii_inv j) i j)) as aij.
                     forward_call.
-                    { rewrite_repr aij. rewrite_repr aii_inv. rewrite_zbits aij. rewrite_zbits aii_inv. 
-                      split; solve_qpoly_bounds. }
-                    { rewrite_repr aij. rewrite_repr aii_inv. rewrite_zbits aij. rewrite_zbits aii_inv.
+                    { unfold FIELD_TABLES. entailer!. }
+                    { simpl_repr. split; solve_qpoly_bounds. } 
+                    { simpl_repr.
                       forward. (*loop invariant preservation*)
                       Exists (j+1). entailer!.
-                      { rewrite arr_field_address0; auto; try lia. rewrite arr_field_address; auto; try lia. f_equal; lia. }
+                      { solve_offset. }
                       { rewrite !poly_of_int_inv. 
                         remember ((get (F:=F) (scalar_mul_row_partial (F:=F)
                         (all_lc_one_rows_partial (F:=F) (gauss_all_steps_rows_partial (F:=F) mx m m) i)i
@@ -912,32 +705,26 @@ Proof.
                          remember ((find_inv mod_poly (get (F:=F)
                          (all_lc_one_rows_partial (F:=F) (gauss_all_steps_rows_partial (F:=F) mx m m) i)
                          i i))) as aii_inv.
-                        rewrite (@scalar_mul_row_plus_1 F _ m n); try lia. 2: solve_wf.
+                        rewrite (@scalar_mul_row_plus_1 F _ m n); [| solve_wf | lia | lia].
                         replace (ssralg.GRing.mul (R:=ssralg.GRing.Field.ringType F)) with  
                           (r_mul mod_poly) by reflexivity. unfold r_mul. unfold poly_mult_mod.
                         rewrite !upd_Znth_map.
-                        rewrite <- (@flatten_mx_set m n); try lia. 2: solve_wf. simpl.
+                        rewrite <- (@flatten_mx_set m n); [|solve_wf | lia | lia]. simpl.
                         rewrite Heqaij. rewrite poly_mult_comm.
-                        rewrite (@scalar_mul_row_outside _ m n); try lia. cancel. solve_wf. }
+                        rewrite (@scalar_mul_row_outside _ m n); try lia; [ unfold FIELD_TABLES; cancel | solve_wf]. }
                     }
                   }
                 }
               }
-              { (*end of outer loop*) forward. Exists (i+1). entailer!.
-                f_equal; unfold Int.zero_ext; f_equal.
-                rewrite unsigned_repr; [rewrite zbits_small; rep_lia | rep_lia].
+              { (*end of outer loop*) forward. Exists (i+1). entailer!. solve_repr_int. reflexivity.
                 rewrite all_lc_one_plus_one; [| lia]. unfold scalar_mul_row.
                 (*need to know that j = n*)
                 assert (Haddr: (field_address (tarray tuchar (m * n)) 
                     [ArraySubsc (i * n + n - 1 - (n - 1))] s) =
-                    (field_address0 (tarray tuchar (m * n)) [ArraySubsc (i * n + n - 1 - (n - 1))] s)). {
-                 rewrite arr_field_address; auto; try lia. rewrite arr_field_address0; auto; try lia. }
+                    (field_address0 (tarray tuchar (m * n)) [ArraySubsc (i * n + n - 1 - (n - 1))] s)) by solve_offset.
                 rewrite Haddr in HRE; clear Haddr.
                 assert (Hjn: j >= n). {
-                  (*TODO: make separate lemma and replace both*)
-                  assert (Hft: forall a b, typed_false a b -> ~(typed_true a b)). { intros a b F T.
-                  unfold typed_true in T; unfold typed_false in F; rewrite T in F; inversion F. }
-                  apply Hft in HRE; clear Hft. rewrite (not_iff_compat) in HRE. 2: {
+                  apply typed_false_not_true in HRE. rewrite (not_iff_compat) in HRE. 2: {
                   rewrite ptr_comparison_gt_iff. reflexivity. all: auto. all: simpl; lia. }
                   lia. } 
                   assert (j = n) by lia. subst; clear Hjn HRE. 
